Cambios

HittingSetToSetCover/HittingSetToSetCover_simple.dfy
@@ -3,6 +3,7 @@ include "../Problems/SetCover.dfy"
 include "../Reductions/ReductionHittingSetToSetCover.dfy"
 include "../Auxiliary/Lemmas.dfy"
 
+
 method HittingSet_to_SetCover_Method(U: set<int>, S: set<set<int>>, k: nat) returns (r:(set<set<int>>, set<set<set<int>>>, nat), ghost counter:nat)
   requires forall s | s in S ::  s <= U
   //ensures r == HittingSet_to_SetCover(U, S, k)
@@ -29,17 +30,17 @@ method HittingSet_to_SetCover_Method(U: set<int>, S: set<set<int>>, k: nat) retu
   var S_contains_empty:bool := false;
   var S' := S;
   counter := counter + |S|;
-  assert counter <= poly1(U, S, k);
+  assert counter <= poly_aux_1(U, S, k);
   while (S' != {})
     decreases |S'|
     invariant S' <= S
     invariant S_contains_empty == ({} in (S - S'))
-    invariant counter <= poly1(U, S, k) + (|S| - |S'|)*(poly_contains_empty_loop(U, S, k) + 1)
+    invariant counter <= poly_aux_1(U, S, k) + (|S| - |S'|)*(poly_contains_empty_loop(U, S, k) + 1)
   {
     counter := counter + 1;
     S', S_contains_empty, counter := HittingSet_to_SetCover_S_contains_empty_loop(U, S, k, S', S_contains_empty, counter);
   }
-  assert counter <= poly1(U, S, k) + |S|*(poly_contains_empty_loop(U, S, k) + 1);
+  assert counter <= poly_aux_1(U, S, k) + |S|*(poly_contains_empty_loop(U, S, k) + 1);
   counter := counter + 1;
 
   if (S_contains_empty) {
@@ -47,25 +48,21 @@ method HittingSet_to_SetCover_Method(U: set<int>, S: set<set<int>>, k: nat) retu
     counter := counter + 1;
     var S' := S;
     counter := counter;
-    //assert counter <= poly1(U, S, k) + |S|*(poly_contains_empty_loop(U, S, k) + 1) + |S| + 1;
-    assert counter <= poly2(U, S, k);
+    assert counter <= poly_aux_2(U, S, k);
     while (S' != {})
       decreases |S'|
       invariant S' <= S
       invariant newS == (set s | s in (S - S') :: {s})
-      invariant counter <= poly2(U, S, k) + (|S| - |S'|)*(poly_edge_case_loop(U, S, k) + 1)
+      invariant counter <= poly_aux_2(U, S, k) + (|S| - |S'|)*(poly_edge_case_loop(U, S, k) + 1)
     {
       counter := counter + 1;
       S', newS, counter := HittingSet_to_SetCover_edge_case_loop(U, S, k, S', newS, counter);
-      //assert counter <= poly2(U, S, k) + (|S| - |S'| - 1)*(poly_edge_case_loop(U, S, k) + 1) + 1 + 2*|S|*|U| + |U|;
     }
-    //assert counter <= poly2(U, S, k) + |S|*(poly_edge_case_loop(U, S, k) + 1);
     counter := counter + 1;
     assert counter <= poly(U, S, k);
     return (S, newS, 0), counter;
   }
   else {
-    //assert counter <= poly1(U, S, k) + |S|*(|S|*|U| + 2*|U| + 1) + 1;
     return (S, newS, k), counter;
   }
 
@@ -75,18 +72,18 @@ method HittingSet_to_SetCover_Method(U: set<int>, S: set<set<int>>, k: nat) retu
 method HittingSet_to_SetCover_outer_loop(U:set<int>, S:set<set<int>>, k:nat, U':set<int>, newS:set<set<set<int>>>, ghost counter_in:nat) returns (U'':set<int>, newS':set<set<set<int>>>, ghost counter:nat)
 // Problem requirements
 requires forall s | s in S ::  s <= U
-// Termination
+// Termination in
 requires U' != {}
 // Invariant in
 requires U' <= U
 requires newS == (set u | u in (U - U') :: (set s | s in S && u in s))
-// Decreases
+// Termination out
 ensures |U''| == |U'| - 1
 // Invariant out
 ensures U'' <= U
 ensures newS' == (set u | u in (U - U'') :: (set s | s in S && u in s))
 // Counter
-ensures counter <= counter_in + poly_outer_loop(U, S, k) // 2*|S|*|S|*|U| + 2*|S|*|U|*|U| + 5*|S|*|U| + 3*|S| + |U| + 2
+ensures counter <= counter_in + poly_outer_loop(U, S, k)
 {
   counter := counter_in;
   var u :| u in U';
@@ -127,12 +124,12 @@ ensures counter <= counter_in + poly_outer_loop(U, S, k) // 2*|S|*|S|*|U| + 2*|S
 method HittingSet_to_SetCover_middle_loop(U:set<int>, S:set<set<int>>, k:nat, S':set<set<int>>, u:int, sets_in_S_that_contain_u:set<set<int>>, ghost counter_in:nat) returns (S'':set<set<int>>, sets_in_S_that_contain_u':set<set<int>>, ghost counter:nat)
 // Problem requirements
 requires forall s | s in S ::  s <= U
-// Termination
+// Termination in
 requires S' != {}
 // Invariant in
 requires S' <= S
 requires sets_in_S_that_contain_u == (set s | s in (S - S') && u in s)
-// Decreases
+// Termination out
 ensures |S''| == |S'| - 1
 // Invariant out
 ensures S'' <= S
@@ -161,21 +158,16 @@ ensures counter <= counter_in + poly_middle_loop(U, S, k)
     s', s_contains_u, counter := HittingSet_to_SetCover_inner_loop(U, S, k, s, s', u, s_contains_u, counter);
   }
   counter := counter + 1;
-  assert counter <= counter_in + poly3(U, S, k) by {
-    //assert counter <= counter_in + |S|*|U| + 2*|U| + (|s| - |s'|)*(|U| + 3) + 1;
+  assert counter <= counter_in + poly_aux_3(U, S, k) by {
     if_smaller_then_less_cardinality(s, U);
-    //assert |s| <= |U|;
-    //assert (|s| - |s'|) <= |U|;
     aux_lemma_1(U, S, k, s, s');
-    //assert (|s| - |s'|)*(|U| + 3) <= (|U|)*(|U| + 3);
-    //assert counter <= counter_in + |S|*|U| + 2*|U| + (|U|)*(|U| + 3) + 1;
   }
 
   if (s_contains_u) {
     sets_in_S_that_contain_u' := sets_in_S_that_contain_u + {s};
     counter := counter + |S|*|U|;
   }
-  assert counter <= counter_in + |S|*|U| + poly3(U, S, k);
+  assert counter <= counter_in + |S|*|U| + poly_aux_3(U, S, k);
   assert counter <= counter_in + poly_middle_loop(U, S, k);
 }
 
@@ -183,12 +175,12 @@ ensures counter <= counter_in + poly_middle_loop(U, S, k)
 method HittingSet_to_SetCover_inner_loop(U:set<int>, S:set<set<int>>, k:nat, s:set<int>, s':set<int>, u:int, s_contains_u:bool, ghost counter_in:nat) returns (s'':set<int>, s_contains_u':bool, ghost counter:nat)
 // Problem requirements
 requires forall s | s in S ::  s <= U
-// Termination
+// Termination in
 requires s' != {}
 // Invariant in
 requires s' <= s
 requires s_contains_u == (u in (s - s'))
-// Decreases
+// Termination out
 ensures |s''| == |s'| - 1
 // Invariant out
 ensures s'' <= s
@@ -214,12 +206,12 @@ ensures counter == counter_in + poly_inner_loop(U, S, k)
 method HittingSet_to_SetCover_S_contains_empty_loop(U:set<int>, S:set<set<int>>, k:nat, S':set<set<int>>, S_contains_empty:bool, ghost counter_in:nat) returns (S'':set<set<int>>, S_contains_empty':bool, ghost counter:nat)
 // Problem requirements
 requires forall s | s in S ::  s <= U
-// Termination
+// Termination in
 requires S' != {}
 // Invariant in
 requires S' <= S
 requires S_contains_empty == ({} in (S - S'))
-// Decreases
+// Termination out
 ensures |S''| == |S'| - 1
 // Invariant out
 ensures S'' <= S
@@ -244,12 +236,12 @@ ensures counter == counter_in + poly_contains_empty_loop(U, S, k)
 method HittingSet_to_SetCover_edge_case_loop(U:set<int>, S:set<set<int>>, k:nat, S':set<set<int>>, newS:set<set<set<int>>>, ghost counter_in:nat) returns (S'':set<set<int>>, newS':set<set<set<int>>>, ghost counter:nat)
 // Problem requirements
 requires forall s | s in S ::  s <= U
-// Termination
+// Termination in
 requires S' != {}
 // Invariant in
 requires S' <= S
 requires newS == (set s | s in (S - S') :: {s})
-// Decreases
+// Termination out
 ensures |S''| == |S'| - 1
 // Invariant out
 ensures S'' <= S
@@ -278,19 +270,19 @@ ghost function O_SSUU_SUUU(U: set<int>, S: set<set<int>>, k: nat) : (o:nat) {
 }
 */
 
-ghost function poly1(U: set<int>, S: set<set<int>>, k: nat) : (o:nat)
+ghost function poly_aux_1(U: set<int>, S: set<set<int>>, k: nat) : (o:nat)
 ensures |S| + |U|*(poly_outer_loop(U, S, k) + 2) + 2 <= o
 {
   2*|S|*|S|*|U|*|U| + 2*|S|*|U|*|U|*|U| + 5*|S|*|U|*|U| + 3*|S|*|U| + |U|*|U| + |S| + 4*|U| + 2
 }
 
-ghost function poly2(U: set<int>, S: set<set<int>>, k: nat) : (o:nat)
-ensures poly1(U, S, k) + |S|*(poly_contains_empty_loop(U, S, k) + 1) + |S| + 1 <= o
+ghost function poly_aux_2(U: set<int>, S: set<set<int>>, k: nat) : (o:nat)
+ensures poly_aux_1(U, S, k) + |S|*(poly_contains_empty_loop(U, S, k) + 1) + |S| + 1 <= o
 {
   2*|S|*|S|*|U|*|U| + 2*|S|*|U|*|U|*|U| + |S|*|S|*|U| + 5*|S|*|U|*|U| + 5*|S|*|U| + |U|*|U| + 3*|S| + 4*|U| + 4
 }
 
-ghost function poly3(U: set<int>, S: set<set<int>>, k: nat) : (o:nat)
+ghost function poly_aux_3(U: set<int>, S: set<set<int>>, k: nat) : (o:nat)
 {
   |S|*|U| + 2*|U| + (|U|)*(|U| + 3) + 1
 }
@@ -301,7 +293,7 @@ ghost function poly_inner_loop(U: set<int>, S: set<set<int>>, k: nat) : (o:nat)
 }
 
 ghost function poly_middle_loop(U: set<int>, S: set<set<int>>, k: nat) : (o:nat)
-  ensures |S|*|U| + poly3(U, S, k) <= o
+  ensures |S|*|U| + poly_aux_3(U, S, k) <= o
 {
   2*|S|*|U| + 2*|U| + |U|*(|U| + 3) + 1
 }
@@ -322,21 +314,13 @@ ghost function poly_edge_case_loop(U: set<int>, S: set<set<int>>, k: nat) : (o:n
 }
 
 ghost function poly(U: set<int>, S: set<set<int>>, k: nat) : (o:nat)
-  //ensures poly1(U, S, k) + |S|*(|S|*|U| + 2*|U| + 1) + 1 <= o
-  ensures poly2(U, S, k) + |S|*(poly_edge_case_loop(U, S, k) + 1) + 1 <= o
+  ensures poly_aux_2(U, S, k) + |S|*(poly_edge_case_loop(U, S, k) + 1) + 1 <= o
 {
-  /*
   calc == {
-    poly1(U, S, k) + |S|*(|S|*|U| + 2*|U| + 1) + 1;
-    poly1(U, S, k) + |S|*|S|*|U| + 2*|S|*|U| + |S| + 1;
-  }
-  */
-
-  calc == {
-    poly2(U, S, k) + |S|*(poly_edge_case_loop(U, S, k) + 1) + 1;
-    poly2(U, S, k) + |S|*(2*|S|*|U| + |U| + 1) + 1;
-    poly2(U, S, k) + 2*|S|*|S|*|U| + |S|*|U| + |S| + 1;
-    poly2(U, S, k) + 2*|S|*|S|*|U| + |S|*|U| + |S| + 1;
+    poly_aux_2(U, S, k) + |S|*(poly_edge_case_loop(U, S, k) + 1) + 1;
+    poly_aux_2(U, S, k) + |S|*(2*|S|*|U| + |U| + 1) + 1;
+    poly_aux_2(U, S, k) + 2*|S|*|S|*|U| + |S|*|U| + |S| + 1;
+    poly_aux_2(U, S, k) + 2*|S|*|S|*|U| + |S|*|U| + |S| + 1;
     (2*|S|*|S|*|U|*|U| + 2*|S|*|U|*|U|*|U| + |S|*|S|*|U| + 5*|S|*|U|*|U| + 5*|S|*|U| + |U|*|U| + 3*|S| + 4*|U| + 4) + 2*|S|*|S|*|U| + |S|*|U| + |S| + 1;
     2*|S|*|S|*|U|*|U| + 2*|S|*|U|*|U|*|U| + 3*|S|*|S|*|U| + 5*|S|*|U|*|U| + 6*|S|*|U| + |U|*|U| + 4*|S| + 4*|U| + 5;
   }
