VerificationSetCover/VerificationSetCover_simple.dfy
@@ -3,17 +3,20 @@ include "../Auxiliary/Lemmas.dfy"
 
 
 method verifySetCover(U:set<int>, S:set<set<int>>, k:nat, I:set<set<int>>) returns (b:bool, ghost counter:nat)   
-requires forall s | s in S :: s <= U
+requires forall s | s in S :: s <= U 
+requires forall s | s in I :: s <= U                  // ???
 ensures b == (I <= S && isCover(U, I) && |I| <= k)
-ensures counter <= poly(U, S, k)
+ensures counter <= poly(U, S, k, I)
 {
   counter := 0;
   var U' := U;
   counter := counter + |U|;
   b:= true;
+  var I_seq_S:bool;
+  I_seq_S, counter := isSubset(U, I, S, counter);
   
   counter := counter + 1;
-  if (!(I <= S && |I| <= k)) {
+  if (!(I_seq_S && |I| <= k)) {
     return false, counter;
   }
 
@@ -21,7 +24,7 @@ ensures counter <= poly(U, S, k)
     decreases |U'|
     invariant U' <= U 
     invariant b == isCover(U-U',I)
-    invariant counter <= |U| + 1 + (|U| - |U'|)*(poly_outer_loop(U, S, k, I) + 1)
+    invariant counter <= |U| + poly_isSubset(U, I, S) + 1 + (|U| - |U'|)*(poly_outer_loop(U, S, k, I) + 1)
   {
     counter := counter + 1;
     b, U', counter := verifySetCover_outer_loop(U, S, k, I, U', counter);
@@ -29,16 +32,64 @@ ensures counter <= poly(U, S, k)
   counter := counter + 1;
   counter_simplification(U, S, k, I, U');
   assert b ==> U-U' == U;
-  b := b;
 }
 
+method isSubset(U:set<int>, S1:set<set<int>>, S2:set<set<int>>, ghost counter_in:nat) returns (b:bool, ghost counter:nat)
+requires forall s |s in S1 :: s <= U
+requires forall s |s in S2 :: s <= U
+ensures b == (S1 <= S2)
+ensures counter <= counter_in + poly_isSubset(U, S1, S2)
+{
+  counter := counter_in;
+  b := true;
+  var S1':= S1;
+  counter := counter + |U|*|S1|;
+  while (S1' != {})
+  // Termination
+  decreases |S1'|
+  // Regular invariants
+  invariant b == ((S1 - S1') <= S2)
+  invariant S1' <= S1
+  // Counter
+  invariant counter <= counter_in + |S1|*|U| + constant + (|S1| - |S1'|)*(poly_isSubset_loop(U, S1, S2) + 1)
+  {
+    S1', b, counter := isSubset_loop(U, S1, S2, S1', counter, b);
+    counter := counter + 1;
+  }
+}
+
+method isSubset_loop(U:set<int>, S1:set<set<int>>, S2:set<set<int>>, S1':set<set<int>>, ghost counter_in:nat, b:bool) returns (S1'':set<set<int>>, b':bool, ghost counter:nat)
+// Termination in
+requires S1' != {}
+// Invariant in
+requires b == ((S1 - S1') <= S2)
+requires S1' <= S1
+// Termination out
+ensures |S1''| == |S1'| - 1
+// Invariant out
+ensures b' == ((S1 - S1'') <= S2)
+ensures S1'' <= S1
+// Counter
+ensures counter <= counter_in + poly_isSubset_loop(U, S1, S2)
+{
+  if_smaller_then_less_cardinality(S1', S1);
+  counter := counter_in;
+  var s:set<int> :| s in S1';
+  counter := counter + |U|;
+  b' := b && s in S2;
+  counter := counter + |S2|*|U|;
+  S1'' := S1' - {s};
+  counter := counter + |S1|*|U|;
+}
+
+
 method verifySetCover_outer_loop(U:set<int>, S:set<set<int>>, k:nat, I:set<set<int>>, U':set<int>, ghost counter_in:nat) returns (b1:bool, U'':set<int>, ghost counter:nat)
-// Termination
+// Termination in
 requires U' != {}
 // Invariant in
 requires U' <= U
 requires isCover(U - U', I)
-// Decreases
+// Termination out
 ensures |U''| == |U'| - 1
 // Invariant out
 ensures U'' <= U
@@ -70,12 +121,12 @@ ensures counter <= counter_in + poly_outer_loop(U, S, k, I)
 
 
 method verifySetCover_inner_loop(U:set<int>, S:set<set<int>>, k:nat, I:set<set<int>>, I':set<set<int>>, u:int, ghost counter_in:nat) returns (b2:bool, I'':set<set<int>>, ghost counter:nat)
-// Termination
+// Termination in
 requires I' != {}
 // Invariant in
 requires I' <= I
 requires !(exists i' | i' in I - I' :: u in i')
-// Decreases
+// Termination out
 ensures |I''| == |I'| - 1
 // Invariant out
 ensures I'' <= I
@@ -96,34 +147,36 @@ lemma counter_simplification(U:set<int>, S:set<set<int>>, k:nat, I:set<set<int>>
 requires forall s | s in S :: s <= U
 requires |I| <= k
 requires U' <= U
-ensures |U| + 2 + (|U| - |U'|)*(1 + |S|*|U| + |U| + 2 + |I|*(|S|*|U| + 2*|U| + 1)) <=
-        (k + 1)*|S|*|U|*|U| + (2*k + 1)*|U|*|U| + (4 + k)*|U| + 2
+ensures |U| + poly_isSubset(U, I, S) + 2 + (|U| - |U'|)*(poly_outer_loop(U, S, k, I) + 1) <= poly(U, S, k, I)
 {
-  assert (1 + k)*|S|*|U|*|U| == (k + 1)*|S|*|U|*|U|;
-  assert |I|*|U|*(|S|*|U| + 2*|U| + 1) <= k*|U|*(|S|*|U| + 2*|U| + 1) by {
-    assert |I|*|U| <= k*|U|;
-  }
   calc <= {
-    |U| + 2 + (|U| - |U'|)*(1 + |S|*|U| + |U| + 2 + |I|*(|S|*|U| + 2*|U| + 1));
-    |U| + 2 + (|U|)*(1 + |S|*|U| + |U| + 2 + |I|*(|S|*|U| + 2*|U| + 1));
-    |U| + 2 + |U| + |S|*|U|*|U| + |U|*|U| + 2*|U| + |I|*|U|*(|S|*|U| + 2*|U| + 1);
-    4*|U| + |S|*|U|*|U| + |U|*|U| + |I|*|U|*(|S|*|U| + 2*|U| + 1) + 2;
-    4*|U| + |S|*|U|*|U| + |U|*|U| + k*|U|*(|S|*|U| + 2*|U| + 1) + 2;
-    4*|U| + |S|*|U|*|U| + |U|*|U| + (k*|U|*|S|*|U| + k*|U|*2*|U| + k*|U|*1) + 2;
-    4*|U| + |S|*|U|*|U| + |U|*|U| + k*|S|*|U|*|U| + 2*k*|U|*|U| + k*|U| + 2;
-    (k + 1)*|S|*|U|*|U| + (2*k + 1)*|U|*|U| + (4 + k)*|U| + 2;
+    |U| + poly_isSubset(U, I, S) + 2 + (|U| - |U'|)*(poly_outer_loop(U, S, k, I) + 1);
+    |U| + poly_isSubset(U, I, S) + 2 + |U|*poly_outer_loop(U, S, k, I) + |U|;
+    |U| + |I|*|I|*|U| + |I|*|S|*|U| + 2*|I|*|U| + |I| + constant + 2 + |U|*poly_outer_loop(U, S, k, I) + |U|;
+    |I|*|I|*|U| + |I|*|S|*|U| + 2*|I|*|U| + |I| + 2*|U| + 3 + |U|*poly_outer_loop(U, S, k, I);
+    |I|*|I|*|U| + |I|*|S|*|U| + 2*|I|*|U| + |I| + 2*|U| + 3 + |U|*(|I|*|S|*|U| + 2*|I|*|U| + |S|*|U| + |I| + |U| + 2);
+    |I|*|I|*|U| + |I|*|S|*|U| + 2*|I|*|U| + |I| + 2*|U| + 3 + |I|*|S|*|U|*|U| + 2*|I|*|U|*|U| + |S|*|U|*|U| + |I|*|U| + |U|*|U| + 2*|U|;
+    |I|*|S|*|U|*|U| + |I|*|I|*|U| + |I|*|S|*|U| + 2*|I|*|U|*|U| + |S|*|U|*|U| + 3*|I|*|U| + |U|*|U| + |I| + 4*|U| + 3;
   }
 }
 
+ghost function poly_isSubset_loop(U: set<int>, S1:set<set<int>>, S2:set<set<int>>) : (o:nat)
+{
+  |S1|*|U| + |S2|*|U| + |U|
+}
+ghost function poly_isSubset(U: set<int>, S1:set<set<int>>, S2:set<set<int>>) : (o:nat)
+{
+  |S1|*|S1|*|U| + |S1|*|S2|*|U| + 2*|S1|*|U| + |S1| + 1
+}
 ghost function poly_inner_loop(U: set<int>, S: set<set<int>>, k: nat) : (o:nat) {
   |S|*|U| + 2*|U|
 }
-
 ghost function poly_outer_loop(U: set<int>, S: set<set<int>>, k: nat, I:set<set<int>>) : (o:nat)
+ensures |S|*|U| + |U| + 2 + |I|*(|S|*|U| + 2*|U| + 1) == o
 {
-  |S|*|U| + |U| + 2 + |I|*(|S|*|U| + 2*|U| + 1)
+  |I|*|S|*|U| + 2*|I|*|U| + |S|*|U| + |I| + |U| + 2
 }
 
-ghost function poly(U: set<int>, S: set<set<int>>, k: nat) : (o:nat) {
-  (k + 1)*|S|*|U|*|U| + (2*k + 1)*|U|*|U| + (4 + k)*|U| + 2
+ghost function poly(U: set<int>, S: set<set<int>>, k: nat, I:set<set<int>>) : (o:nat) {
+  |I|*|S|*|U|*|U| + |I|*|I|*|U| + |I|*|S|*|U| + 2*|I|*|U|*|U| + |S|*|U|*|U| + 3*|I|*|U| + |U|*|U| + |I| + 4*|U| + 3
 }
